Some polish, some extra rewrite tools, some patches to receive loop, a little bit more work done on ffi_irrel proof, and beginning to character receive_loop correctness

projection/proofs/lib_tools/evaluate_rwLib.sig
@@ -4,4 +4,5 @@ sig
 	val trans_sl:thm list
 	val eval_sl_nf:thm list
 	val eval_sl:thm list
+	val eval_sl_nffi:thm list
 end
